lemmas partially admitted

code/experimental/P256/Hacl.Spec.P256.Lemmas.fst
@@ -22,15 +22,6 @@ let log_and a b =
   UInt.logand_commutative #(bits U64) (v a) (v b)
 
 noextract
-val logor_zeros: a:uint64 -> Lemma (uint_v (a `logor` (u64 0)) == uint_v a)
-
-let logor_zeros a = 
-  UInt.logor_lemma_1 #(bits U64) (v a);
-  assert(UInt.logor #(bits U64) (v a) 0 = (v a))
-  
-
-
-noextract
 val log_or: a: uint64 -> b: uint64 {uint_v b == 0 \/ uint_v a == 0} -> 
 Lemma (if uint_v b = 0 then uint_v (logor a b) == uint_v a else uint_v (logor a b) == uint_v b)
 
@@ -282,6 +273,7 @@ val lemma_reduce_mod_by_sub2: t: nat ->
   Lemma ((prime256 * (t % pow2 64)) % pow2 64 == (-t)  % pow2 64)
 
 let lemma_reduce_mod_by_sub2 t = 
+  admit();
   let t_ = t % pow2 64 in   
   let f = (pow2 256 - pow2 224 + pow2 192 + pow2 96 -1) * (t % pow2 64) in 
   assert(f == pow2 256 * t_ - pow2 224 * t_ + pow2 192 * t_ + pow2 96 * t_ - t_);
@@ -351,7 +343,8 @@ val lemma_reduce_mod_ecdsa_prime:
 let lemma_reduce_mod_ecdsa_prime prime t k0 = 
     let open FStar.Tactics in 
     let open FStar.Tactics.Canon in 
-  
+
+admit();
   let f = prime * (k0 * (t % pow2 64) % pow2 64) in 
   let t0 = (t + f) % pow2 64 in 
   lemma_mod_add_distr t f (pow2 64);
@@ -405,6 +398,7 @@ val lemma_decrease_pow: a: nat -> Lemma (ensures (a * modp_inv2 (pow2 64) * modp
 
 
 let lemma_decrease_pow a = 
+  admit();
   assert_norm(modp_inv2 (pow2 64) = 6277101733925179126845168871924920046849447032244165148672);
   assert_norm(pow2 256 = 115792089237316195423570985008687907853269984665640564039457584007913129639936);
   assert_norm(modp_inv2 (pow2 256) =115792089183396302114378112356516095823261736990586219612555396166510339686400 );
@@ -497,9 +491,9 @@ val lemma_xor_copy_cond: a: uint64 -> b: uint64 -> mask: uint64{uint_v mask = 0 
   if uint_v mask = pow2 64 - 1 then r == b else r == a)
 
 
-val lognot_lemma: #t:inttype{~(U1? t)} -> a:uint_t t SEC -> Lemma
-  (requires v a = 0 \/ v a = maxint t)
-  (ensures (if v a = 0 then v (lognot a) == maxint t else v (lognot a) == 0)) 
+val lognot_lemma: a:uint_t U64 SEC -> Lemma
+  (requires v a = 0 \/ v a = maxint U64)
+  (ensures (if v a = 0 then v (lognot a) == maxint U64 else v (lognot a) == 0)) 
 
 
 val lemma_equality: a: felem4 -> b: felem4 -> Lemma
@@ -509,9 +503,9 @@ val lemma_equality: a: felem4 -> b: felem4 -> Lemma
 
       if  (uint_v a_0 = uint_v b_0 && uint_v a_1 = uint_v b_1 && uint_v a_2 = uint_v b_2 && uint_v a_3 = uint_v b_3) then as_nat4 a == as_nat4 b else as_nat4 a <> as_nat4 b)
 
- val neq_mask_lemma: #t:inttype -> a:uint_t t SEC -> b:uint_t t SEC -> Lemma
+assume val neq_mask_lemma: a:uint_t U64 SEC -> b:uint_t U64 SEC -> Lemma
   (requires True)
-  (ensures  (v a <> v b ==> v (neq_mask a b) == maxint t) /\
+  (ensures  (v a <> v b ==> v (neq_mask a b) == maxint U64) /\
             (v a == v b ==> v (neq_mask a b) == 0))
 
 
@@ -566,6 +560,7 @@ let lemma_distr_mult7 a b c d e f h = admit()
 
 
 let lemma_prime_as_wild_nat a =
+  admit();
    assert_norm(pow2 64 * pow2 64 = pow2 128);
    assert_norm(pow2 64 * pow2 64 * pow2 64 = pow2 192);
    assert_norm(pow2 64 * pow2 64 * pow2 64 * pow2 64 = pow2 256);
@@ -623,12 +618,9 @@ let lemma_xor_copy_cond a b mask =
     logxor_lemma a snd;
     logxor_lemma a b
 
-let lognot_lemma #t a = admit()
+let lognot_lemma a = admit()
 
 let lemma_equality a b = ()
-
-let neq_mask_lemma #t a b = admit()
-
 
 let cmovznz4_lemma cin x y = 
   let x2 = neq_mask cin (u64 0) in 
